trying to show that contextual closure is wf ... not sure it is true

gore.v
@@ -14,6 +14,148 @@ Require Import utils acc perm_eq mso mpo.
 
 Notation "'⟨' x '|' l '⟩ₜ'" := (node x l) (at level 0, l at level 200, format "⟨ x | l ⟩ₜ").
 
+(** Notations for the construction of the list order *)
+#[local] Reserved Notation "x '≺' y" (at level 70, no associativity, format "x  ≺  y").
+#[local] Reserved Notation "x '≺ₗ' y" (at level 70, no associativity, format "x  ≺ₗ  y").
+#[local] Reserved Notation "x '⊏' y" (at level 70, no associativity, format "x  ⊏  y").
+#[local] Reserved Notation "x '⊏⁺' y" (at level 70, no associativity, format "x  ⊏⁺  y").
+
+#[local] Hint Constructors clos_trans : core.
+#[local] Hint Resolve Acc_inv Acc_intro 
+                      in_cons in_eq in_elt in_or_app : core.
+Section list_order.
+
+  Variables (X : Type) (R : X → X → Prop).
+
+  Infix "≺" := R.
+  Notation "l ≺ₗ y" := (∀x, x ∈ l → x ≺ y).
+
+  Local Fact lt_fall_sg x y : x ≺ y → [x] ≺ₗ y.
+  Proof. now intros ? ? [ <- | [] ]. Qed.
+
+  Hint Resolve lt_fall_sg : core.
+
+  (* Inductive definition of the list relation ⊏ 
+     of which the transitive closure ⊏⁺ is the list order. *)
+
+  Inductive lo_step : list X → list X → Prop :=
+    | lo_step_intro l x y r : x ≺ y → l++[x]++r ⊏ l++[y]++r
+  where "l ⊏ m" := (lo_step l m).
+
+  Hint Constructors lo_step : core.
+
+  Fact lo_step_ctx l r u v : u ⊏ v → l++u++r ⊏ l++v++r.
+  Proof.
+    induction 1 in l, r |- *; eauto.
+    rewrite <- !app_assoc, !(app_assoc l); eauto.
+  Qed.
+
+  (* The inversion lemma gives an alternate characterization,
+     used below for more specific inversion lemmas below *)
+  Local Fact lo_step_inv k p :
+         k ⊏ p ↔ ∃ l x y r, k = l++[x]++r ∧ p = l++[y]++r ∧ x ≺ y.
+  Proof.
+    split.
+    + intros [ l m x r ]; now exists l, m, x, r.
+    + intros (? & ? & ? & ? & -> & -> & ?); eauto.
+  Qed.
+
+  (** These two are key lemmas in the proof of (Acc lo_step) below *)
+
+  Local Fact lo_step_nil_inv l : ~ l ⊏ [].
+  Proof. now intros ([] & ? & ? & ? & ? & ? & ?)%lo_step_inv. Qed.
+
+  Local Lemma lo_step_cons_right_inv k y m : 
+          k ⊏ y::m 
+        → (∃ x, k = x::m ∧ x ≺ y)
+        ∨ (∃ l u x r, m = l++[x]++r ∧ k = y::l++[u]++r ∧ u ≺ x).
+  Proof.
+    intros ([ | z l] & u & x & r & hk & e & hu)%lo_step_inv; simpl in *;
+    apply cons_inj in e as [-> ->]; [ left | right ]; eauto.
+    exists l, u, x, r; eauto.
+  Qed.
+
+  Section Acc_lo_step.
+
+    Notation W := (Acc lo_step).
+
+    Local Fact Acc_lo_step_nil : W [].
+    Proof. constructor 1; intros _ []%lo_step_nil_inv. Qed.
+
+    Local Fact W_app_bound y r :
+        (∀x, x ≺ y → ∀l, W l → W (x::l))
+       → W r 
+       → ∀l, l ≺ₗ y → W (l++r).
+    Proof.
+      intros hy ? l. 
+      induction l; simpl; eauto.
+      intros; apply hy; eauto.
+    Qed.
+
+    Hint Resolve W_app_bound : core.
+
+    Local Fact W_cons_rec y m :
+           (∀x, x ≺ y → ∀l, W l → W (x::l))
+         → W m
+         → (∀l, l ⊏ m → W (y::l))
+         → W (y::m).
+    Proof. constructor; intros ? [ (? & -> & ?) | (? & ? & ? & ? & -> & -> & ?) ]%lo_step_cons_right_inv; eauto. Qed.
+
+    Hint Resolve W_cons_rec : core.
+
+    Local Fact W_cons y : (∀x, x ≺ y → ∀l, W l → W (x::l)) → ∀l, W l → W (y::l).
+    Proof. induction 2; eauto. Qed.
+
+    Hint Resolve W_cons : core.
+
+    Local Lemma Acc_lo_step_cons x : Acc R x → ∀l, W l → W (x::l).
+    Proof. induction 1; eauto. Qed.
+
+  End Acc_lo_step.
+
+  Hint Resolve Acc_lo_step_nil
+               Acc_lo_step_cons : core.
+
+  (* W is closed under [] and x::_ for any accessible x
+     so it contains any list composed of accessibles *) 
+  Lemma forall_Acc_lo_step l : (∀x, x ∈ l → Acc R x) → Acc lo_step l.
+  Proof.
+    rewrite <- Forall_forall.
+    induction 1; eauto.
+  Qed.
+
+  Lemma Acc_lo_step_forall l : Acc lo_step l → ∀x, x ∈ l → Acc R x.
+  Proof.
+    induction 1 as [ m _ IH ]; intros y (l & r & ->)%in_split.
+    constructor 1; intros x Hx.
+    apply IH with (l++[x]++r); auto.
+  Qed.
+
+  Hint Resolve forall_Acc_lo_step Acc_lo_step_forall : core.
+
+  Theorem Acc_lo_step_iff l : Acc lo_step l ↔ ∀x, x ∈ l → Acc R x.
+  Proof. split; eauto. Qed.
+
+End list_order.
+
+Arguments lo_step {_}.
+
+(*
+Section mono.
+
+  Variables (X : Type) (R T : X → X → Prop).
+
+  Fact lo_step_mono : R ⊆₂ T → lo_step R ⊆₂ lo_step T.
+  Proof. induction 2; constructor; eauto. Qed.
+
+  Hint Resolve lo_step_mono : core.
+
+  Fact lo_mono : R ⊆₂ T → lo R ⊆₂ lo T.
+  Proof. intro; apply clos_trans_mono; eauto. Qed.
+
+End mono.
+*)
+
 Section ctxt.
 
   Variables (X : Type).
@@ -27,14 +169,28 @@ Section ctxt.
 
   Fact ctxt_inv R p q : 
       ctxt R p q 
-    → R p q \/ exists f l r u v , p = ⟨f|l++[u]++r⟩ₜ /\ q = ⟨f|l++[v]++r⟩ₜ /\ ctxt R u v.
+    → R p q ∨ ∃ f l r u v, p = ⟨f|l++[u]++r⟩ₜ ∧ q = ⟨f|l++[v]++r⟩ₜ ∧ ctxt R u v.
   Proof.
     destruct 1; eauto.
     right; do 5 eexists; eauto.
-  Qed. 
-  
-  Fact Acc_fall R f m : Acc R ⟨f|m⟩ₜ → Forall (Acc (ctxt R)) m → Acc (ctxt R) ⟨f|m⟩ₜ.
+  Qed.
+
+  Variables (R : _) (R_wf : well_founded R). 
+
+  Fact Acc_fall t : Forall (Acc (ctxt R)) (sons t) → Acc (ctxt R) t.
   Proof.
+    rewrite -> Forall_forall, <- Acc_lo_step_iff.
+    induction t as [ [f m] IH ] using (well_founded_induction R_wf).
+    simpl; intros Hm.
+    constructor.
+    intros s [ | ]%ctxt_inv; eauto.
+    + apply IH; auto.
+    change m with (sons ⟨f|m⟩ₜ) at 2.
+    generalize ⟨f|m⟩ₜ; clear f m.
+    induction 1 as [ [f m] _ IH1 ]; simpl.
+    induction 1 as [ m _ IH2 ].
+    
+    + apply IH1; auto.
   Admitted.
   
   Fact wf_ctxt R : well_founded R → well_founded (ctxt R).
@@ -44,12 +200,6 @@ Section ctxt.
     rewrite <- Forall_forall in IHm.
     apply Acc_fall; auto.
   Qed.
-    constructor.
-    intros ? [ | (g & l & r & p & q & -> & [=] & G)]%ctxt_inv; eauto.
-    subst g m.
-    apply IHm.
-    
-    
 
   Hint Constructors ctxt : core.
   
@@ -68,7 +218,7 @@ Section ctxt.
   
   Fact sn1__sn2 r t : sn1 r t → sn2 r t.
   Proof. now constructor 1. Qed.
-  
+  (*
   
   
   
@@ -76,3 +226,4 @@ Section ctxt.
     | sn1_intro f l p q r : SN q → ctxt p q → sn1 ⟨f|l++[p]++r⟩ₜ ⟨f|l++[q]++r⟩ₜ.
     
     (node f ()) (node f (l++[p]++r))
+*)
